examples/Online_with_authn/DY.OnlineA.Run.Printing.fst
@@ -1,15 +1,13 @@
-module DY.OnlineS.Run.Printing
+module DY.OnlineA.Run.Printing
 
 open DY.Core
 open DY.Lib
 open Comparse
 
-open DY.Simplified
-
-open DY.OnlineS.Data
+open DY.OnlineA.Data
 
 /// Helper functions for trace printing.
-/// Here we define how our abstract message and state types
+/// Here we define how our abstract message, state and event types
 /// should be printed.
 
 val message_to_string: bytes -> option string
@@ -25,10 +23,17 @@ let state_to_string b =
   | SentAck a -> Some (Printf.sprintf "SentAck [n_a = (%s), to = (%s)]" (bytes_to_string a.n_a) a.alice)
   | ReceivedAck r -> Some (Printf.sprintf "ReceivedAck [n_a = (%s), from = (%s)]" (bytes_to_string r.n_a) r.bob)
 
+val event_to_string: bytes -> option string
+let event_to_string b =
+  match? parse event_t b with
+  | Initiating {alice; bob; n_a} -> Some (Printf.sprintf "Initiating [alice = (%s), n_a = (%s), to = (%s)]" alice (bytes_to_string n_a) bob)
+  | Responding {alice; bob; n_a} -> Some (Printf.sprintf "Responding [bob = (%s), n_a = (%s), to = (%s)]" bob (bytes_to_string n_a) alice)
+  | Finishing {alice; bob; n_a} -> Some (Printf.sprintf "Finishing [alice = (%s), n_a = (%s), with = (%s)]" alice (bytes_to_string n_a) bob)
+  
 
 val get_trace_to_string_printers: trace_to_string_printers
 let get_trace_to_string_printers  = 
   trace_to_string_printers_builder 
     message_to_string
-    ((local_state_state_t.tag, state_to_string) :: default_state_to_string)
-    []
+    [(local_state_state_t.tag, state_to_string)]
+    [(event_event_t.tag, event_to_string)]
