examples/Online_with_secrecy/DY.OnlineS.Invariants.Proofs.fst
@@ -192,7 +192,7 @@ let send_ping_invariant alice bob alice_private_keys_sid  tr =
          bob is stored in the first component of the state.
          So the state prediate is satisfied:
       *)
-      assert(state_predicate_p.pred tr_msg alice sid st);
+      assert(state_predicate_online.pred tr_msg alice sid st);
       (* With this, we have all pre-conditions of `set_state_invariant`.
          Since that lemma comes with an SMT pattern,
          it is applied automatically.
@@ -208,20 +208,19 @@ let send_ping_invariant alice bob alice_private_keys_sid  tr =
    we end up with the following very short proof.
 *)
 val send_ping_invariant_short_version:
-  alice:principal -> bob:principal -> alice_private_keys_sid:state_id ->
+  alice:principal -> bob:principal -> alice_public_keys_sid:state_id ->
   tr:trace ->
   Lemma
-  ( requires trace_invariant tr
-  )
+  (requires trace_invariant tr)
   (ensures (
-    let (_ , tr_out) = send_ping alice bob alice_private_keys_sid tr in
+    let (_ , tr_out) = send_ping alice bob alice_public_keys_sid tr in
     trace_invariant tr_out
   ))
-let send_ping_invariant_short_version alice bob alice_private_keys_sid  tr =
+let send_ping_invariant_short_version alice bob alice_public_keys_sid tr =
   let (n_a, tr_rand) = gen_rand_labeled (nonce_label alice bob) tr in
   let ping = Ping {alice; n_a} in 
   serialize_wf_lemma message_t (is_knowable_by (nonce_label alice bob) tr_rand) ping;
-  pke_enc_for_is_publishable tr_rand alice bob alice_private_keys_sid key_tag ping
+  pke_enc_for_is_publishable tr_rand alice bob alice_public_keys_sid key_tag ping
 
 
 (*** Replying to a Ping maintains the invariants ***)
@@ -251,22 +250,14 @@ val decode_ping_proof:
   msg:bytes ->
   Lemma
   (requires (
-    trace_invariant tr
-    /\ bytes_invariant tr msg
+    trace_invariant tr /\
+    bytes_invariant tr msg
   ))
   (ensures (
     match decode_ping bob bob_private_keys_sid msg tr with
     | (None, _) -> True
-    | (Some png, _) -> (
-        let n_a = png.n_a in
-        let (sk_bob, _) = get_private_key bob bob_private_keys_sid (LongTermPkeKey key_tag) tr in
-        Some? sk_bob /\
-        bytes_invariant tr n_a /\
-        is_knowable_by (nonce_label png.alice bob) tr n_a /\
-        ( is_publishable tr n_a
-        \/ (pke_pred.pred tr (long_term_key_type_to_usage (LongTermPkeKey key_tag) bob) (pk (Some?.v sk_bob)) (serialize message_t (Ping png)))
-        )
-    )
+    | (Some {alice; n_a}, _) ->
+        is_knowable_by (nonce_label alice bob) tr n_a
   ))
 let decode_ping_proof tr bob bob_private_keys_sid msg =
     match decode_ping bob bob_private_keys_sid msg tr with
@@ -279,15 +270,13 @@ let decode_ping_proof tr bob bob_private_keys_sid msg =
     )
   
 
-
 /// The invariant lemma for the `receive_ping_and_send_ack` step
 
 val receive_ping_and_send_ack_invariant:
   bob:principal -> bob_private_keys_sid:state_id -> bob_public_keys_sid:state_id -> ts:timestamp ->
   tr:trace ->
   Lemma
-  ( requires trace_invariant tr
-  )
+  (requires trace_invariant tr)
   (ensures (
     let (_ , tr_out) = receive_ping_and_send_ack bob bob_private_keys_sid bob_public_keys_sid ts tr in
     trace_invariant tr_out
@@ -322,8 +311,8 @@ let receive_ping_and_send_ack_invariant bob bob_private_keys_sid bob_public_keys
              //       tr_out == tr )
              //    = () in
           
-          let n_a = png.n_a in
           let alice = png.alice in
+          let n_a = png.n_a in
           
           let ack = Ack {n_a} in
           
@@ -385,13 +374,12 @@ let receive_ping_and_send_ack_invariant bob bob_private_keys_sid bob_public_keys
 
                    We get this property from our helper lemma `decode_ping_proof`.
                 *)
-                let st = (SentAck {alice = png.alice; n_a = png.n_a}) in
+                let st = (SentAck {alice; n_a}) in
                 let (sess_id, tr_sess) = start_new_session bob st tr_msg in
                 assert(trace_invariant tr_sess)
            )
       )
   )
-
 
 
 (*** Receiving an Ack maintains the invariants ***)
@@ -400,14 +388,12 @@ val decode_ack_invariant:
   alice:principal -> alice_private_keys_sid:state_id -> cipher:bytes ->
   tr:trace ->
   Lemma
-  (requires
-    trace_invariant tr
-  )
+  (requires trace_invariant tr)
   (ensures (
     let (_, tr_out) = decode_ack alice alice_private_keys_sid cipher tr in
     trace_invariant tr_out
   ))
-let decode_ack_invariant alice keys_sid msg tr = ()
+let decode_ack_invariant alice alice_private_keys_sid msg tr = ()
 
 
 /// The invariant lemma for the final protocol step `receive_ack_invariant`
@@ -417,9 +403,7 @@ val receive_ack_invariant:
   alice:principal -> alice_private_keys_sid:state_id -> msg_ts:timestamp ->
   tr:trace ->
   Lemma
-  (requires
-    trace_invariant tr
-  )
+  (requires trace_invariant tr)
   (ensures (
     let (_, tr_out) = receive_ack alice alice_private_keys_sid msg_ts tr in
     trace_invariant tr_out
