examples/Online/DY.Online.Run.Printing.fst
@@ -12,13 +12,11 @@ open DY.Online.Data
 /// Here we define how our abstract message and state types
 /// should be printed.
 
-
 val message_to_string: bytes -> option string
 let message_to_string b =
   match? parse message_t b with
   | Ping p -> Some (Printf.sprintf "Ping [name = (%s), n_a = (%s)]" (p.alice) (bytes_to_string p.n_a))
   | Ack a -> Some (Printf.sprintf "Ack [n_a = (%s)]" (bytes_to_string a.n_a))
-
 
 val state_to_string: bytes -> option string
 let state_to_string b =
@@ -32,5 +30,5 @@ val get_trace_to_string_printers: trace_to_string_printers
 let get_trace_to_string_printers  = 
   trace_to_string_printers_builder 
     message_to_string
-    ((local_state_state.tag, state_to_string) :: default_state_to_string)
+    ((local_state_state_t.tag, state_to_string) :: default_state_to_string)
     []
