examples/Online_with_authn/DY.OnlineA.Data.fst
@@ -1,0 +1,149 @@
+module DY.OnlineA.Data
+
+open Comparse
+open DY.Core
+open DY.Lib
+
+/// Here, we define the abstract types for the "Online?" Protocol:
+///
+/// A -> B: enc{Ping (A, n_A)}_B
+/// B -> A: enc{Ack n_A}_A
+///
+/// (They are the same as for the simple 2 message protocol)
+
+
+/// We only highlight the differences to the previous model
+/// for showing nonce secrecy.
+
+(*** Message Type ***)
+
+[@@ with_bytes bytes]
+type ping_t = {
+  alice: principal;
+  n_a : bytes;
+}
+
+[@@ with_bytes bytes]
+type ack_t = {
+  n_a : bytes;
+}
+
+/// the overall abstract message type
+
+[@@ with_bytes bytes]
+type message_t =
+  | Ping: (ping:ping_t) -> message_t
+  | Ack: (ack:ack_t) -> message_t
+
+%splice [ps_ping_t] (gen_parser (`ping_t))
+
+%splice [ps_ack_t] (gen_parser (`ack_t))
+
+%splice [ps_message_t] (gen_parser (`message_t))
+
+instance parseable_serializeable_bytes_message_t: parseable_serializeable bytes message_t = mk_parseable_serializeable ps_message_t
+
+
+(*** State Type ***)
+
+[@@ with_bytes bytes]
+type sent_ping_t = {
+  bob : principal;
+  n_a : bytes;
+}
+
+[@@ with_bytes bytes]
+type sent_ack_t = {
+  alice: principal;
+  n_a : bytes;
+}
+
+[@@ with_bytes bytes]
+type received_ack_t = {
+  bob : principal;
+  n_a : bytes;
+}
+
+[@@ with_bytes bytes]
+type state_t = 
+  | SentPing: (ping:sent_ping_t) -> state_t
+  | SentAck: (ack:sent_ack_t) -> state_t
+  | ReceivedAck: (rack:received_ack_t) -> state_t
+
+%splice [ps_sent_ping_t] (gen_parser (`sent_ping_t))
+%splice [ps_sent_ack_t] (gen_parser (`sent_ack_t))
+%splice [ps_received_ack_t] (gen_parser (`received_ack_t))
+%splice [ps_state_t] (gen_parser (`state_t))
+
+instance parseable_serializeable_bytes_state_t: parseable_serializeable bytes state_t = mk_parseable_serializeable ps_state_t
+
+instance local_state_state_t: local_state state_t = {
+  tag = "Online.State";
+  format = parseable_serializeable_bytes_state_t;
+}
+
+
+
+(*** PKI ***)
+
+let key_tag = "Online.Key"
+
+
+(*** Event type ***)
+
+/// We are now using events to show the authentication property.
+/// We have one event for each protocol step,
+/// that is
+/// * an Initiating event, that Alice triggers, when she starts a new run
+/// * a Responding event, that Bob triggers, when he replies to a Ping with an Ack
+/// * and a Finishing event, that Alice triggers, when she finishes a run.
+/// 
+/// Just as for messages and states,
+/// we define abstract event types
+
+/// The abstract type of the Initiating event
+[@@ with_bytes bytes]
+type ev_init_t = {
+  alice:principal;
+  bob:principal;
+  n_a:bytes
+}
+
+/// The abstract type of the Responding event
+[@@ with_bytes bytes]
+type ev_respond_t = {
+  alice:principal;
+  bob:principal;
+  n_a:bytes
+}
+
+/// The abstract type of the Finishing event
+[@@ with_bytes bytes]
+type ev_finish_t = {
+  alice:principal;
+  bob:principal;
+  n_a:bytes
+}
+
+
+/// The overall event type
+[@@ with_bytes bytes]
+type event_t =
+  | Initiating: ev_init_t -> event_t
+  | Responding: ev_respond_t -> event_t
+  | Finishing: ev_finish_t -> event_t
+
+
+/// Using Comparse to generate parser and serializer for the abstract event types
+%splice [ps_ev_init_t] (gen_parser (`ev_init_t))
+%splice [ps_ev_respond_t] (gen_parser (`ev_respond_t))
+%splice [ps_ev_finish_t] (gen_parser (`ev_finish_t))
+%splice [ps_event_t] (gen_parser (`event_t))
+%splice [ps_event_t_is_well_formed] (gen_is_well_formed_lemma (`event_t))
+
+
+/// Make the overall event type an instance of DY.Lib event class
+instance event_event_t: event event_t = {
+  tag = "Online.Event";
+  format = mk_parseable_serializeable ps_event_t;
+}
