examples/Online_with_authn/DY.OnlineA.Invariants.fst
@@ -1,0 +1,244 @@
+module DY.OnlineA.Invariants
+
+open Comparse 
+open DY.Core
+open DY.Lib
+open DY.Extend
+
+open DY.OnlineA.Data
+open DY.OnlineA.Protocol
+
+#set-options "--fuel 0 --ifuel 1 --z3rlimit 25"
+
+/// In this module, we define the protocol invariants.
+/// They consist of
+/// * crypto invariants and
+/// * trace invariants which in turn consist of
+///   * state invariants and
+///   * event invariants
+///
+/// We then have to show
+/// * these invariants imply the secrecy property (see DY.OnlineS.Secrecy) and
+/// * every protocol step maintains these invariants (see DY.OnlineS.Invariants.Proofs)
+/// With this, we then know that
+/// the protocol model satisfies the secrecy property.
+
+/// We only highlight the differences to the previous model
+/// for showing nonce secrecy.
+
+(*** Crypto Invariants ***)
+
+
+%splice [ps_ping_t_is_well_formed] (gen_is_well_formed_lemma (`ping_t))
+%splice [ps_ack_t_is_well_formed] (gen_is_well_formed_lemma (`ack_t))
+%splice [ps_message_t_is_well_formed] (gen_is_well_formed_lemma (`message_t))
+
+instance crypto_usages_online : crypto_usages = default_crypto_usages
+
+#push-options "--ifuel 3"
+let crypto_predicates_online : crypto_predicates = { 
+  default_crypto_predicates with 
+  pke_pred = { 
+    pred = (fun tr sk_usage pk msg ->
+    exists prin. (
+      sk_usage == long_term_key_type_to_usage (LongTermPkeKey key_tag) prin /\
+      (match parse message_t msg with
+      | Some (Ping {alice; n_a}) ->
+          let bob = prin in
+          get_label tr n_a == nonce_label alice bob
+
+          (* We add, that the Alice specified in the Ping message,
+             must have triggered an Initiating event
+             with 
+             * her own name (alice)
+             * the intended receiver of the Ping (bob) and
+             * the nonce n_a in the Ping
+          *)
+          /\ event_triggered tr alice (Initiating {alice; bob; n_a})
+      | Some (Ack {n_a}) ->
+          (* For nonce secrecy,
+             we didn't have any conditions/guarantees in the Ack case.
+             Now, we add that 
+             some Bob must have triggered a Responding event with
+             * the intended receiver of the Ack (alice)
+             * his own name (bob) and
+             * the nonce (n_a) in the Ack
+          *)
+          let alice = prin in
+          exists bob. event_triggered tr bob (Responding {alice; bob; n_a})
+      | _ -> False
+      ))
+      ); 
+    pred_later = (fun tr1 tr2 sk_usage pk msg -> 
+      parse_wf_lemma message_t (bytes_well_formed tr1) msg
+    ) 
+  } 
+}
+#pop-options
+
+/// Collecting the usages and prediates in the final crypto invariants
+
+instance crypto_invariants_online: crypto_invariants = {
+  usages = crypto_usages_online;
+  preds =  crypto_predicates_online
+}
+
+
+(*** State Invariant ***)
+
+%splice [ps_sent_ping_t_is_well_formed] (gen_is_well_formed_lemma (`sent_ping_t))
+%splice [ps_sent_ack_t_is_well_formed] (gen_is_well_formed_lemma (`sent_ack_t))
+%splice [ps_received_ack_t_is_well_formed] (gen_is_well_formed_lemma (`received_ack_t))
+%splice [ps_state_t_is_well_formed] (gen_is_well_formed_lemma (`state_t))
+
+#push-options "--ifuel 2 --z3cliopt 'smt.qi.eager_threshold=50'"
+let state_predicate_online: local_state_predicate state_t = {
+  pred = (fun tr prin sess_id st ->
+    match st with
+    | SentPing {bob; n_a} -> (
+        let alice = prin in
+        is_secret (nonce_label alice bob) tr n_a
+        (* We add, that the storing principal (alice),
+           must have triggered an Initiating event with:
+           * her own name
+           * the bob stored in the state and
+           * the nonce stored in the state
+        *)
+        /\ event_triggered tr alice (Initiating {alice; bob; n_a})
+    )
+    | SentAck {alice; n_a} -> (
+        let bob = prin in
+        is_knowable_by (principal_label bob) tr n_a
+        (* Additionally, we enforce that
+           the storing principal (bob) 
+           must have triggered e Responding event with:
+           * the stored name (alice)
+           * his own name (bob)
+           * the stored nonce (n_a)
+        *)
+        /\ event_triggered tr bob (Responding {alice; bob; n_a})
+    )
+    | ReceivedAck {bob; n_a}  -> (
+        let alice = prin in
+        is_secret (nonce_label alice bob) tr n_a
+
+        (* We add, that the storing principal (alice),
+          must have triggered a Finishing event with:
+          * her own name
+          * the bob stored in the state and
+          * the nonce stored in the state
+        *)
+        /\ event_triggered tr alice (Finishing {alice; bob; n_a})
+    )
+  );
+  pred_later = (fun tr1 tr2 prin sess_id st -> () );
+  pred_knowable = (fun tr prin sess_id st -> () );
+}
+#pop-options
+
+
+(*** Event Predicates ***)
+
+/// As for messages and states,
+/// we also have predicates on events.
+/// The intuition is similar:
+/// They say when an event is allowed to be triggered, or
+/// what guarantees we obtain, if we observe a specific event on the trace.
+
+let event_predicate_online: event_predicate event_t =
+  fun tr prin e ->
+  // prin is the principal triggering the event
+    match e with    
+    | Initiating {alice; bob; n_a} -> (
+        (* We may trigger the Initiating event only if,
+           * the triggering principal is the first principal stored in the event (alice)
+           * the nonce (n_a) in the event is labelled for 
+             the two principals stored in the event (alice and bob)
+           * the stored nonce (n_a) was generated right before the event is triggered
+             (this is crucial and will be used to show an injectivity property,
+             that there will be only one such event for a fixed nonce n_a)
+        *)
+        prin == alice /\
+        is_secret (nonce_label alice bob) tr n_a /\
+        rand_just_generated tr n_a
+    )
+    | Responding {alice; bob; n_a} -> (
+        (* A Responding event may only be triggered if,
+           * the triggering principal is the second principal stored in the event (bob)
+           * if the stored nonce n_a has not leaked,
+             then the first stored principal (alice)
+             must have triggered an Initiating event with the same data
+             as the Responding event
+        *)
+        prin == bob /\ 
+        ( is_publishable tr n_a \/
+          event_triggered tr alice (Initiating {alice; bob; n_a}))
+    )
+    | Finishing {alice; bob; n_a} -> (
+        (* A Finishing event may only be triggered if,
+           * the triggering principal is the first principal stored in the event (alice)
+           * the same principal triggered an Initiating event with the same bob and n_a
+           * if the stored nonce n_a has not leaked,
+             then the second stored principal (bob)
+             must have triggered a Responding event with the same data
+        *)
+        prin == alice /\
+        event_triggered tr alice (Initiating {alice; bob; n_a}) /\
+        ( is_publishable tr n_a \/
+          event_triggered tr bob (Responding {alice; bob; n_a}))
+    )
+
+
+(*** Trace invariants ***)
+
+let all_sessions = [
+  pki_tag_and_invariant;
+  private_keys_tag_and_invariant;
+  (|local_state_state_t.tag, local_state_predicate_to_local_bytes_state_predicate state_predicate_online|);
+]
+
+/// Now we have an event type
+let all_events = [(event_event_t.tag, compile_event_pred event_predicate_online)]
+
+let trace_invariants_online: trace_invariants = {
+  state_pred = mk_state_pred all_sessions;
+  event_pred = mk_event_pred all_events;
+}
+
+
+(*** Protocol Invariants ***)
+
+instance protocol_invariants_online: protocol_invariants = {
+  crypto_invs = crypto_invariants_online;
+  trace_invs = trace_invariants_online;
+}
+
+/// Lemmas that the global state predicate contains all the local ones
+
+val all_sessions_has_all_sessions: unit -> Lemma (norm [delta_only [`%all_sessions; `%for_allP]; iota; zeta] (for_allP (has_local_bytes_state_predicate) all_sessions))
+let all_sessions_has_all_sessions () =
+  assert_norm(List.Tot.no_repeats_p (List.Tot.map dfst (all_sessions)));
+  mk_state_pred_correct all_sessions;
+  norm_spec [delta_only [`%all_sessions; `%for_allP]; iota; zeta] (for_allP (has_local_bytes_state_predicate) all_sessions)
+
+val protocol_invariants_p_has_p_session_invariant: squash (has_local_state_predicate state_predicate_online)
+let protocol_invariants_p_has_p_session_invariant = all_sessions_has_all_sessions ()
+
+val protocol_invariants_p_has_pki_invariant: squash (has_pki_invariant #protocol_invariants_online)
+let protocol_invariants_p_has_pki_invariant = all_sessions_has_all_sessions ()
+
+val protocol_invariants_p_has_private_keys_invariant: squash (has_private_keys_invariant #protocol_invariants_online)
+let protocol_invariants_p_has_private_keys_invariant = all_sessions_has_all_sessions ()
+
+/// Lemmas that the global event predicate contains all the local ones
+
+val all_events_has_all_events: unit -> Lemma (norm [delta_only [`%all_events; `%for_allP]; iota; zeta] (for_allP (has_compiled_event_pred #protocol_invariants_online) all_events))
+let all_events_has_all_events () =
+  assert_norm(List.Tot.no_repeats_p (List.Tot.map fst (all_events)));
+  mk_event_pred_correct #protocol_invariants_online all_events;
+  norm_spec [delta_only [`%all_events; `%for_allP]; iota; zeta] (for_allP (has_compiled_event_pred #protocol_invariants_online) all_events);
+  let dumb_lemma (x:prop) (y:prop): Lemma (requires x /\ x == y) (ensures y) = () in
+  dumb_lemma (for_allP (has_compiled_event_pred #protocol_invariants_online) all_events) (norm [delta_only [`%all_events; `%for_allP]; iota; zeta] (for_allP (has_compiled_event_pred #protocol_invariants_online) all_events))
+
+val protocol_invariants_p_has_event_t_invariant: squash (has_event_pred event_predicate_online)
+let protocol_invariants_p_has_event_t_invariant = all_events_has_all_events ()
